\documentclass{article}
\usepackage{amsfonts}
\usepackage{amsmath}
\usepackage{indentfirst}

\title{Mathematical analysis. Lesson 8. Homework}
\author{Plyuhin Aleksandr}
\date{}

\begin{document}
\maketitle

\section{} 
    $ z = \sqrt{1-x^3} + \ln{(y^2-1)} $
    
    $
    \begin{cases}
      1-x^3 \geq 0 \\
      y^2-1>0
    \end{cases}
    \begin{cases}
      1 \geq x^3 \\
      y^2>1
    \end{cases}
    \begin{cases}
      x \leq 1 \\
      y>1
    \end{cases}
    $

\section{}
    $ z = \left( 1 + \frac{\ln{x}}{\ln{y}} \right)^3 $
    
    
    $ z'_x = \left( \left( 1 + \frac{\ln{x}}{\ln{y}} \right)^3 \right)'_x = $
    $ 3 \left( 1 + \frac{\ln{x}}{\ln{y}} \right)^2   \left( 1 + \frac{\ln{x}}{\ln{y}} \right)'_x  = $
    
    $ = 3 \left( 1 + \frac{\ln{x}}{\ln{y}} \right)^2 \frac{1}{\ln{y}} \frac{1}{x} = $
    $ \frac{3}{x\ln{y}}  \left( 1 + \frac{\ln{x}}{\ln{y}} \right)^2 $
    
    
    $ z'_y = \left( \left( 1 + \frac{\ln{x}}{\ln{y}} \right)^3 \right)'_y = $
    $ 3 \left( 1 + \frac{\ln{x}}{\ln{y}} \right)^2   \left( 1 + \frac{\ln{x}}{\ln{y}} \right)'_y  = $
    
    $ = 3 \left( 1 + \frac{\ln{x}}{\ln{y}} \right)^2   \ln{x} \cdot \left( (\ln{y})^{-1} \right)'_y = $
    
    $ = 3 \left( 1 + \frac{\ln{x}}{\ln{y}} \right)^2   \ln{x} \cdot (-1)(\ln{y})^{-2} \cdot \frac{1}{y} = $
    
    $ = -\frac{3\ln{x}}{y(\ln{y})^2}   \left( 1 + \frac{\ln{x}}{\ln{y}} \right)^2 $

\section{}
    $ z = \sqrt{2xy + \cos{\frac{x}{y}}} $
    
    
    $ z'_x = \left(  (2xy + \cos{\frac{x}{y}}) ^ {\frac{1}{2}} \right)'_x = $
    $ \frac{1}{2} (2xy + \cos{\frac{x}{y}}) ^ {-\frac{1}{2}}  (2xy + \cos{\frac{x}{y}})'_x= $
    
    $ = \frac{1}{2} (2xy + \cos{\frac{x}{y}}) ^ {-\frac{1}{2}}  (2y - \sin{\frac{x}{y}} \cdot \frac{1}{y}) $
    
    
    $ z'_y = \left(  (2xy + \cos{\frac{x}{y}}) ^ {\frac{1}{2}} \right)'_y = $
    $ \frac{1}{2} (2xy + \cos{\frac{x}{y}}) ^ {-\frac{1}{2}}  (2xy + \cos{\frac{x}{y}})'_y= $
    
    $ = \frac{1}{2} (2xy + \cos{\frac{x}{y}}) ^ {-\frac{1}{2}}  (2x - \sin{\frac{x}{y}} \cdot x(-1)y^{-2}) $
    
    
    $ dz = z'_x dx + z'_y dy = $
    
    $ = \frac{ 2y -\frac{1}{y} \sin{\frac{x}{y}} }{ 2\sqrt{2xy+\cos{\frac{x}{y}}} } dx + $
    $ \frac{ 2x +\frac{x}{y^2} \sin{\frac{x}{y}} }{ 2\sqrt{2xy+\cos{\frac{x}{y}}} } dy $
    
    $ dz(1;1) = $
    $ \frac{ 2 -\sin{1} }{ 2\sqrt{2+\cos{1}} } dx + $
    $ \frac{ 2 +\sin{1} }{ 2\sqrt{2+\cos{1}} } dy $

\section{}
    $ z = x^2 + xy + y^2 -6x -9y $
    
    $ z'_x = 2x+y-6 $
    
    $ z'_y = x+2y-9 $
    
    $ z''_{xx} = 2 $
    
    $ z''_{yy} = 2 $
    
    $ z''_{xy} = 1 $
    
    $ z''_{yx} = 1 $

    $
    \begin{cases}
      2x+y-6=0 \\
      x+2y-9=0
    \end{cases}
    \begin{cases}
      y=6-2x \\
      x+2(6-2x)-9=0
    \end{cases}
    $

    $
    \begin{cases}
      y=6-2x \\
      -3x+3=0
    \end{cases}
    \begin{cases}
      y=6-2=4 \\
      x=1
    \end{cases}
    $
    
    M(1;4)
    
    $ \Delta = 
    \begin{vmatrix}
    z''_{xx} & z''_{xy} \\
    z''_{xy} & z''_{yy} 
    \end{vmatrix}
    = z''_{xx} z''_{yy} - (z''_{xy})^2 = 2 \cdot 2 -1 = 3 >0
    $
    
    $ z''_{xx} > 0 $
    
    M(1;4) is local minimum

\end{document}