\documentclass{article}
\usepackage{amsfonts}
\usepackage{amsmath}
\usepackage{indentfirst}

\title{Mathematical analysis. Lesson 6. Homework}
\author{Plyuhin Aleksandr}
\date{}

\begin{document}
\maketitle

\section{} 
    \subsection{}
        $
        y' = (\sin{x} \cdot \cos{x})' = (\sin{x})' \cdot \cos{x} + \sin{x}(\cos{x})' =
        \cos^2{x} - \sin^2{x}
        $
    
    \subsection{}
        $
        y' = \left( \ln{(2x+1)^3} \right)' = \frac{ \left( (2x+1)^3 \right)' }{(2x+1)^3} =
        \frac{3(2x+1)^2 \cdot 2}{(2x+1)^3} = \frac{6}{2x+1}
        $
    
    \subsection{}
        $
        y' = \left( \sqrt{\sin^2{(\ln{x^3})}} \right)' =
        \left( \left| \sin{(\ln{x^3})} \right| \right)' =
        \frac{\sin{(\ln{x^3})}} {\left| \sin{(\ln{x^3})} \right|} \left( \sin{(\ln{x^3})} \right)' =*
        $
        
        $
        \left( \sin{(\ln{x^3})} \right)' =
        \left( \cos{(\ln{x^3})} \right) \cdot (\ln{x^3})' =
        \left( \cos{(\ln{x^3})} \right) \cdot \frac{1}{x^3} \cdot (x^3)' =
        
         \cos{(\ln{x^3})}  \cdot \frac{1}{x^3} \cdot 3x^2 =
        \cos{(\ln{x^3})}  \cdot \frac{3}{x}
        $
        
        $
        *= \frac{3 \cdot \sin{(\ln{x^3})} \cdot \cos{(\ln{x^3})}} 
                {x \cdot \left| \sin{(\ln{x^3})} \right|}
        $
    
    \subsection{}
        $
        y' = \left( \frac{x^4}{\ln{x}} \right)' =
        \left( x^4 \cdot (\ln{x})^{-1} \right)' =
        \frac{(x^4)'}{\ln{x}} + x^4 \left((\ln{x})^{-1} \right)' =
        $
        
        $
        \frac{4x^3}{\ln{x}} + x^4 (-1) (\ln{x})^{-2} (\ln{x})' =
        \frac{4x^3}{\ln{x}} + \frac{x^4}{\ln^2{x}} \cdot \frac{1}{x} =
        \frac{4x^3}{\ln{x}} + \frac{x^4}{x\ln^2{x}}
        $

\section{}
    $
    f'(x) = \left( \cos{(x^2+3x)} \right)' =
    -\sin{(x^2+3x)} \cdot (x^2+3x)' =
    $
    
    $
    =-\sin{(x^2+3x)}(2x+3)
    $
    
    $
    f'(\sqrt{\pi}) = - (2\sqrt{\pi}+3) \sin{(\pi+3\sqrt{\pi})}
    $

\section{}
    $
    f'(x) = \left( (x^3-x^2-x-1)(1+2x+3x^2-4x^3)^{-1} \right)' =
    $
    
    $
    \frac{(x^3-x^2-x-1)'} {1+2x+3x^2-4x^3} + (x^3-x^2-x-1)(-1)(1+2x+3x^2-4x^3)^{-2}(1+2x+3x^2-4x^3)' =
    $
    
    $
    \frac{3x^2-2x-1} {1+2x+3x^2-4x^3} - \frac{x^3-x^2-x-1} {(1+2x+3x^2-4x^3)^2}
    (2+6x-12x^2)
    $
    
    $
    f'(0) = \frac{-1}{1} - \frac{-1}{1} (2) = -1+2 = 1
    $

\section{}
    $
    f'(x) = \left( (3x)^{\frac{1}{2}} \ln{x} \right)'
    = \left( (3x)^{\frac{1}{2}} \right)' \ln{x} + \sqrt{3x}(\ln{x})' =
    $
    
    $
    = \frac{1}{2} (3x)^{-\frac{1}{2}} (3x)' \ln{x} + \frac{\sqrt{3x}}{x}
    = \frac{3\ln{x}} {2\sqrt{3x}} + \frac{\sqrt{3x}}{x}
    = \frac{3x\ln{x} + 6x} {2x\sqrt{3x}}
    = \frac{3\ln{x} + 6} {2\sqrt{3x}}
    $
    
    $
    f'(1) = \frac{3\ln{1}+6} {2\sqrt{3}}
    $

\end{document}